SyBloc/SBIsDefined.v
@@ -1,0 +1,95 @@
+Require Import Velus.Common.
+Require Import Velus.Operators.
+Require Import Velus.NLustre.NLExprSyntax.
+Require Import Velus.SyBloc.SBSyntax.
+Require Import Velus.Clocks.
+
+Require Import Velus.SyBloc.SBIsVariable.
+Require Import Velus.SyBloc.SBIsLast.
+
+Require Import List.
+Import List.ListNotations.
+Open Scope list_scope.
+
+Module Type SBISDEFINED
+       (Import Ids     : IDS)
+       (Import Op      : OPERATORS)
+       (Import Clks    : CLOCKS       Ids)
+       (Import ExprSyn : NLEXPRSYNTAX     Op)
+       (Import Syn     : SBSYNTAX     Ids Op Clks ExprSyn)
+       (Import Var     : SBISVARIABLE Ids Op Clks ExprSyn Syn)
+       (Import Last    : SBISLAST     Ids Op Clks ExprSyn Syn).
+
+  Inductive Is_defined_in_eq: ident -> equation -> Prop :=
+  | DefEqDef:
+      forall x ck e,
+        Is_defined_in_eq x (EqDef x ck e)
+  | DefEqNext:
+      forall x ck e,
+        Is_defined_in_eq x (EqNext x ck e)
+  | DefEqCall:
+      forall x s xs ck rst b es,
+        In x xs ->
+        Is_defined_in_eq x (EqCall s xs ck rst b es).
+
+  Definition Is_defined_in (x: ident) (eqs: list equation) : Prop :=
+    Exists (Is_defined_in_eq x) eqs.
+
+  Lemma Is_defined_Is_variable_Is_last_in:
+    forall eqs x,
+      Is_defined_in x eqs ->
+      Is_variable_in x eqs \/ Is_last_in x eqs.
+  Proof.
+    induction eqs; inversion_clear 1 as [?? Def|?? Defs].
+    - inv Def.
+      + left; left; constructor; auto.
+      + right; left; constructor; auto.
+      + left; left; constructor; auto.
+    - apply IHeqs in Defs as [].
+      + left; right; auto.
+      + right; right; auto.
+  Qed.
+
+  Lemma b_ins_not_def:
+    forall b x,
+      InMembers x b.(b_in) ->
+      ~ Is_defined_in x b.(b_eqs).
+  Proof.
+    intros ** Hin Hdef.
+    pose proof (b_nodup b) as Nodup.
+    eapply (NoDup_app_In x) in Nodup.
+    - apply Is_defined_Is_variable_Is_last_in in Hdef as [Var|Last];
+        apply Nodup, in_app.
+      + apply Is_variable_in_variables in Var; rewrite <-b_vars_out_in_eqs in Var;
+          auto.
+      + apply lasts_of_In in Last; rewrite <-b_lasts_in_eqs in Last; auto.
+    - apply fst_InMembers; auto.
+  Qed.
+
+  Lemma not_Is_defined_in_eq_EqDef:
+    forall y x ck e,
+      ~ Is_defined_in_eq y (EqDef x ck e) -> x <> y.
+  Proof.
+    intros ** NIsDef E; subst; apply NIsDef; auto using Is_defined_in_eq.
+  Qed.
+
+  Lemma not_Is_defined_in_eq_EqNext:
+    forall y x ck e,
+      ~ Is_defined_in_eq y (EqNext x ck e) -> x <> y.
+  Proof.
+    intros ** NIsDef E; subst; apply NIsDef; auto using Is_defined_in_eq.
+  Qed.
+
+  Lemma not_Is_defined_in_cons:
+    forall x eq eqs,
+      ~ Is_defined_in x (eq :: eqs)
+      <-> ~ Is_defined_in_eq x eq /\ ~ Is_defined_in x eqs.
+  Proof.
+    split.
+    - intro Hndef; split; intro His_def;
+        eapply Hndef; constructor (assumption).
+    - intros [Hdef_eq Hdef_eqs] Hdef_all.
+      inv Hdef_all; eauto.
+  Qed.
+
+End SBISDEFINED.
