SyBloc/SBIsFree.v
@@ -1,0 +1,44 @@
+Require Import Velus.Common.
+Require Import Velus.Operators.
+Require Import Velus.NLustre.NLExprSyntax.
+Require Import Velus.SyBloc.SBSyntax.
+Require Import Velus.Clocks.
+
+Require Import Velus.NLustre.NLSyntax.
+Require Export Velus.NLustre.IsFree.
+
+Require Import List.
+Import List.ListNotations.
+Open Scope list_scope.
+
+Module Type SBISFREE
+       (Import Ids     : IDS)
+       (Import Op      : OPERATORS)
+       (Import Clks    : CLOCKS       Ids)
+       (Import ExprSyn : NLEXPRSYNTAX     Op)
+       (Import Syn     : SBSYNTAX     Ids Op Clks ExprSyn)
+       (SynNL          : NLSYNTAX     Ids Op Clks ExprSyn)
+       (Import IsF     : ISFREE       Ids Op Clks ExprSyn SynNL).
+
+  Inductive Is_free_in_eq: ident -> equation -> Prop :=
+  | FreeEqDef:
+      forall x ck e y,
+        Is_free_in_caexp y ck e ->
+        Is_free_in_eq y (EqDef x ck e)
+  | FreeEqNext:
+      forall x ck e y,
+        Is_free_in_laexp y ck e ->
+        Is_free_in_eq y (EqNext x ck e)
+  | FreeEqReset:
+      forall s ck b x,
+        Is_free_in_clock x ck ->
+        Is_free_in_eq x (EqReset s ck b)
+  | FreeEqCall:
+      forall s x ck rst b es y,
+        Is_free_in_laexps y ck es ->
+        Is_free_in_eq y (EqCall s x ck rst b es).
+
+  Definition Is_free_in (x: ident) (eqs: list equation) : Prop :=
+    Exists (Is_free_in_eq x) eqs.
+
+End SBISFREE.
