SyBloc/SBIsLast.v
@@ -1,0 +1,89 @@
+Require Import Velus.Common.
+Require Import Velus.Operators.
+Require Import Velus.NLustre.NLExprSyntax.
+Require Import Velus.SyBloc.SBSyntax.
+Require Import Velus.Clocks.
+
+Require Import List.
+Import List.ListNotations.
+Open Scope list_scope.
+
+Module Type SBISLAST
+       (Import Ids     : IDS)
+       (Import Op      : OPERATORS)
+       (Import Clks    : CLOCKS       Ids)
+       (Import ExprSyn : NLEXPRSYNTAX     Op)
+       (Import Syn     : SBSYNTAX     Ids Op Clks ExprSyn).
+
+  Inductive Is_last_in_eq: ident -> equation -> Prop :=
+    LastEqNext:
+      forall x ck e,
+        Is_last_in_eq x (EqNext x ck e).
+
+  Definition Is_last_in (x: ident) (eqs: list equation) : Prop :=
+    Exists (Is_last_in_eq x) eqs.
+
+  Lemma not_Is_last_in_cons:
+    forall x eq eqs,
+      ~ Is_last_in x (eq :: eqs) <-> ~ Is_last_in_eq x eq /\ ~ Is_last_in x eqs.
+  Proof.
+    split; intros HH.
+    - split; intro; apply HH; unfold Is_last_in; intuition.
+    - destruct HH; inversion_clear 1; intuition.
+  Qed.
+
+  Lemma lasts_of_In:
+    forall eqs x,
+      Is_last_in x eqs <-> In x (lasts_of eqs).
+  Proof.
+    induction eqs as [|[]]; simpl.
+    - now setoid_rewrite Exists_nil.
+    - setoid_rewrite <-IHeqs; split; try right; auto.
+      inversion_clear 1 as [?? Last|]; try inv Last; auto.
+    - setoid_rewrite <-IHeqs; split.
+      + inversion_clear 1 as [?? Last|]; try inv Last; auto.
+      + intros [E|?].
+        * subst; left; constructor.
+        * right; auto.
+    - setoid_rewrite <-IHeqs; split; try right; auto.
+      inversion_clear 1 as [?? Last|]; try inv Last; auto.
+    - setoid_rewrite <-IHeqs; split; try right; auto.
+      inversion_clear 1 as [?? Last|]; try inv Last; auto.
+  Qed.
+
+  Definition is_last_in_eq_b (x: ident) (eq: equation) : bool :=
+    match eq with
+    | EqNext y ck e => ident_eqb x y
+    | _ => false
+    end.
+
+  Definition is_last_in_b (x: ident) (eqs: list equation) : bool :=
+    existsb (is_last_in_eq_b x) eqs.
+
+  Fact Is_last_in_eq_reflect:
+    forall x eq,
+      Is_last_in_eq x eq <-> is_last_in_eq_b x eq = true.
+  Proof.
+    destruct eq; simpl; split;
+      try discriminate; try now inversion 1.
+    - inversion_clear 1; apply ident_eqb_refl.
+    - rewrite ident_eqb_eq; intro; subst; constructor.
+  Qed.
+
+  Corollary Is_last_in_reflect:
+    forall x eqs,
+      Is_last_in x eqs <-> is_last_in_b x eqs = true.
+  Proof.
+    setoid_rewrite existsb_exists; setoid_rewrite Exists_exists.
+    split; intros (?&?& Last); apply Is_last_in_eq_reflect in Last; eauto.
+  Qed.
+
+  Lemma Is_last_in_dec:
+    forall x eqs,
+      { Is_last_in x eqs } + { ~ Is_last_in x eqs }.
+  Proof.
+    intros;
+      eapply Bool.reflect_dec, Bool.iff_reflect, Is_last_in_reflect.
+  Qed.
+
+End SBISLAST.
