SyBloc/SBIsVariable.v
@@ -1,0 +1,89 @@
+Require Import Velus.Common.
+Require Import Velus.Operators.
+Require Import Velus.NLustre.NLExprSyntax.
+Require Import Velus.SyBloc.SBSyntax.
+Require Import Velus.Clocks.
+
+Require Import List.
+Import List.ListNotations.
+Open Scope list_scope.
+
+Module Type SBISVARIABLE
+       (Import Ids     : IDS)
+       (Import Op      : OPERATORS)
+       (Import Clks    : CLOCKS       Ids)
+       (Import ExprSyn : NLEXPRSYNTAX     Op)
+       (Import Syn     : SBSYNTAX     Ids Op Clks ExprSyn).
+
+  Inductive Is_variable_in_eq: ident -> equation -> Prop :=
+  | VarEqDef:
+      forall x ck e,
+        Is_variable_in_eq x (EqDef x ck e)
+  | VarEqCall:
+      forall x s xs ck rst b es,
+        In x xs ->
+        Is_variable_in_eq x (EqCall s xs ck rst b es).
+
+  Definition Is_variable_in (x: ident) (eqs: list equation) : Prop :=
+    Exists (Is_variable_in_eq x) eqs.
+
+  Lemma Is_variable_in_variables:
+    forall eqs x,
+      Is_variable_in x eqs <-> In x (variables eqs).
+  Proof.
+    unfold variables, concatMap.
+    induction eqs as [|[]]; simpl.
+    - split; try contradiction; inversion 1.
+    - split.
+      + inversion_clear 1 as [?? Var|]; try inv Var; auto.
+        right; apply IHeqs; auto.
+      + intros [E|].
+        * subst; left; constructor.
+        * right; apply IHeqs; auto.
+    - setoid_rewrite <-IHeqs; split.
+      + inversion_clear 1 as [?? Var|]; auto; inv Var.
+      + right; auto.
+    - setoid_rewrite <-IHeqs; split.
+      + inversion_clear 1 as [?? Var|]; auto; inv Var.
+      + right; auto.
+    - split.
+      + inversion_clear 1 as [?? Var|]; try inv Var.
+        * apply in_app; auto.
+        * apply in_app; right; apply IHeqs; auto.
+      + rewrite in_app; intros [?|?].
+        * left; constructor; auto.
+        * right; apply IHeqs; auto.
+  Qed.
+
+  Definition is_variable_in_eq_b (x: ident) (eq: equation) : bool :=
+    match eq with
+    | EqDef x' _ _ => ident_eqb x x'
+    | EqCall _ xs _ _ _ _ => existsb (ident_eqb x) xs
+    | _ => false
+    end.
+
+  Fact Is_variable_in_eq_reflect:
+    forall x eq,
+      Is_variable_in_eq x eq <-> is_variable_in_eq_b x eq = true.
+  Proof.
+    destruct eq; simpl; split;
+      try discriminate; try now inversion 1.
+    - inversion_clear 1; apply ident_eqb_refl.
+    - rewrite ident_eqb_eq; intro; subst; constructor.
+    - inversion_clear 1.
+      apply existsb_exists; eexists; split; eauto.
+      apply ident_eqb_refl.
+    - rewrite existsb_exists; intros (?&?& E).
+      apply ident_eqb_eq in E; subst.
+      constructor; auto.
+  Qed.
+
+  Lemma Is_variable_in_eq_dec:
+    forall x eq,
+      { Is_variable_in_eq x eq } + { ~ Is_variable_in_eq x eq }.
+  Proof.
+    intros;
+      eapply Bool.reflect_dec, Bool.iff_reflect, Is_variable_in_eq_reflect.
+  Qed.
+
+End SBISVARIABLE.
