SyBloc/SBWellDefined.v
@@ -1,0 +1,210 @@
+Require Import Velus.Common.
+Require Import Velus.Operators.
+Require Import Velus.NLustre.NLExprSyntax.
+Require Import Velus.SyBloc.SBSyntax.
+Require Import Velus.Clocks.
+
+Require Import Velus.SyBloc.SBIsBlock.
+Require Import Velus.SyBloc.SBOrdered.
+
+Require Import Velus.SyBloc.SBIsVariable.
+Require Import Velus.SyBloc.SBIsLast.
+Require Import Velus.SyBloc.SBIsDefined.
+
+Require Import Velus.NLustre.NLSyntax.
+Require Import Velus.SyBloc.SBIsFree.
+
+Require Import List.
+Import List.ListNotations.
+Open Scope list_scope.
+
+Module Type SBWELLDEFINED
+       (Import Ids     : IDS)
+       (Import Op      : OPERATORS)
+       (Import Clks    : CLOCKS       Ids)
+       (Import ExprSyn : NLEXPRSYNTAX     Op)
+       (Import Syn     : SBSYNTAX     Ids Op Clks ExprSyn)
+       (Import Block   : SBISBLOCK    Ids Op Clks ExprSyn Syn)
+       (Import Ord     : SBORDERED    Ids Op Clks ExprSyn Syn Block)
+       (Import Var     : SBISVARIABLE Ids Op Clks ExprSyn Syn)
+       (Import Last    : SBISLAST     Ids Op Clks ExprSyn Syn)
+       (Import Def     : SBISDEFINED  Ids Op Clks ExprSyn Syn Var Last)
+       (SynNL          : NLSYNTAX     Ids Op Clks ExprSyn)
+       (Import IsF     : ISFREE       Ids Op Clks ExprSyn     SynNL)
+       (Import Free    : SBISFREE     Ids Op Clks ExprSyn Syn SynNL IsF).
+
+  Inductive Is_well_sch (inputs: list ident) (mems: PS.t): list equation -> Prop :=
+  | WSchNil:
+      Is_well_sch inputs mems []
+  | WSchEq:
+      forall eq eqs,
+        Is_well_sch inputs mems eqs ->
+        (forall x,
+            Is_free_in_eq x eq ->
+            if PS.mem x mems
+            then ~ Is_defined_in x eqs
+            else Is_variable_in x eqs \/ In x inputs) ->
+        (forall x, Is_defined_in_eq x eq -> ~ Is_defined_in x eqs) ->
+        (forall s k,
+            Is_state_in_eq s k eq ->
+            Forall (fun eq => forall k', Is_state_in_eq s k' eq -> k' < k) eqs) ->
+        Is_well_sch inputs mems (eq :: eqs).
+
+  Inductive Well_scheduled: program -> Prop :=
+    | Well_scheduled_nil:
+        Well_scheduled []
+    | Well_scheduled_cons:
+        forall bl P,
+          Well_scheduled P ->
+          Is_well_sch (map fst (b_in bl)) (ps_from_list (map fst (b_lasts bl))) (b_eqs bl) ->
+          Well_scheduled (bl :: P).
+
+  Definition Well_defined (P: program) : Prop :=
+    Ordered_blocks P /\ Well_scheduled P.
+
+  Lemma Is_well_sch_app:
+    forall mems inputs eqs eqs',
+      Is_well_sch mems inputs (eqs ++ eqs') ->
+      Is_well_sch mems inputs eqs'.
+  Proof.
+    induction eqs; auto; simpl.
+    inversion 1; auto.
+  Qed.
+
+  Lemma Reset_not_Step_in:
+    forall eqs inputs mems s ck b,
+      Is_well_sch inputs mems (EqReset s ck b :: eqs) ->
+      ~ Step_in s eqs.
+  Proof.
+    inversion_clear 1 as [|????? States].
+    unfold Step_in, Is_state_in.
+    rewrite Exists_exists.
+    intros (eq' & Hin & IsStin).
+    assert (Forall (fun eq => forall k', Is_state_in_eq s k' eq -> k' < 0) eqs)
+      by (apply States; auto using Is_state_in_eq).
+    eapply Forall_forall in Hin; eauto.
+    apply Hin in IsStin.
+    omega.
+  Qed.
+
+  Lemma Reset_not_Reset_in:
+    forall eqs inputs mems s ck b,
+      Is_well_sch inputs mems (EqReset s ck b :: eqs) ->
+      ~ Reset_in s eqs.
+  Proof.
+    inversion_clear 1 as [|????? States].
+    unfold Reset_in, Is_state_in.
+    rewrite Exists_exists.
+    intros (eq' & Hin & IsStin).
+    assert (Forall (fun eq => forall k', Is_state_in_eq s k' eq -> k' < 0) eqs)
+      by (apply States; auto using Is_state_in_eq).
+    eapply Forall_forall in Hin; eauto.
+    apply Hin in IsStin.
+    omega.
+  Qed.
+
+  Inductive Step_with_reset_spec: list equation -> Prop :=
+  | Step_with_reset_nil:
+      Step_with_reset_spec []
+  | Step_with_reset_EqDef:
+      forall x ck e eqs,
+        Step_with_reset_spec eqs ->
+        Step_with_reset_spec (EqDef x ck e :: eqs)
+  | Step_with_reset_EqNext:
+      forall x ck e eqs,
+        Step_with_reset_spec eqs ->
+        Step_with_reset_spec (EqNext x ck e :: eqs)
+  | Step_with_reset_EqReset:
+      forall s ck b eqs,
+        Step_with_reset_spec eqs ->
+        Step_with_reset_spec (EqReset s ck b :: eqs)
+  | Step_with_reset_EqCall:
+      forall s xs ck (rst: bool) b es eqs,
+        Step_with_reset_spec eqs ->
+        (if rst then Reset_in s eqs else ~ Reset_in s eqs) ->
+        Step_with_reset_spec (EqCall s xs ck rst b es :: eqs).
+
+  Lemma Step_with_reset_spec_app:
+    forall eqs eqs',
+      Step_with_reset_spec (eqs ++ eqs') ->
+      Step_with_reset_spec eqs'.
+  Proof.
+    induction eqs; auto; simpl.
+    inversion 1; auto.
+  Qed.
+
+  Lemma Step_not_Step_Reset_in:
+    forall eqs inputs mems s ys ck rst b es,
+      Is_well_sch inputs mems (EqCall s ys ck rst b es :: eqs) ->
+      Step_with_reset_spec (EqCall s ys ck rst b es :: eqs) ->
+      ~ Step_in s eqs
+      /\ if rst then Reset_in s eqs else ~ Reset_in s eqs.
+  Proof.
+    inversion_clear 1 as [|????? States].
+    inversion_clear 1.
+    split; auto.
+    setoid_rewrite Exists_exists.
+    intros (eq' & Hin & IsStin).
+    assert (Forall (fun eq => forall k', Is_state_in_eq s k' eq -> k' < 1) eqs)
+        by (apply States; auto using Is_state_in_eq).
+    eapply Forall_forall in Hin; eauto.
+    apply Hin in IsStin.
+    omega.
+  Qed.
+
+  Lemma Is_well_sch_Step_with_reset_spec:
+    forall eqs inputs mems,
+      (forall s rst, Step_with_reset_in s rst eqs ->
+                if rst then Reset_in s eqs else ~ Reset_in s eqs) ->
+      Is_well_sch inputs mems eqs ->
+      Step_with_reset_spec eqs.
+  Proof.
+    induction eqs as [|[]]; intros ** Spec WSCH;
+      inversion_clear WSCH as [|??? Free Def States];
+      constructor;
+      clear Free Def;
+      try (eapply IHeqs; eauto; intros ** Step; specialize (Spec s rst));
+      try (setoid_rewrite Step_with_reset_in_cons_not_call in Spec; [|discriminate]).
+    - apply Spec in Step.
+      destruct rst.
+      + inversion_clear Step as [?? Step'|]; auto; inv Step'.
+      + intro; apply Step; right; auto.
+    - apply Spec in Step.
+      destruct rst.
+      + inversion_clear Step as [?? Step'|]; auto; inv Step'.
+      + intro; apply Step; right; auto.
+    - assert (s <> i).
+      { assert (Is_state_in_eq i 0 (EqReset i c i0)) as State by constructor.
+        apply States in State.
+        eapply Forall_Exists, Exists_exists in State as (?&?& StateSpec & Step_eq); eauto.
+        inv Step_eq; intro; subst.
+        assert (1 < 0) by (apply StateSpec; constructor).
+        omega.
+      }
+      apply Spec in Step.
+      destruct rst.
+      + inversion_clear Step as [?? Step'|]; auto; inv Step'.
+        congruence.
+      + intro; apply Step; right; auto.
+    - assert (s <> i).
+      { assert (Is_state_in_eq i 1 (EqCall i i0 c b i1 l)) as State by constructor.
+        apply States in State.
+        eapply Forall_Exists, Exists_exists in State as (?&?& StateSpec & Step_eq); eauto.
+        inv Step_eq; intro; subst.
+        assert (1 < 1) by (apply StateSpec; constructor).
+        omega.
+      }
+      rewrite Step_with_reset_in_cons_call in Spec; auto.
+      apply Spec in Step.
+      destruct rst.
+      + inversion_clear Step as [?? Step'|]; auto; inv Step'.
+      + intro; apply Step; right; auto.
+    - assert (Step_with_reset_in i b (EqCall i i0 c b i1 l :: eqs)) as Step
+          by (left; constructor).
+      apply Spec in Step.
+      destruct b.
+      + inversion_clear Step as [?? Step'|]; auto; inv Step'.
+      + intro; apply Step; right; auto.
+  Qed.
+
+End SBWELLDEFINED.
