SyBlocToObc/SBMemoryCorres.v
@@ -1,0 +1,341 @@
+Require Import Velus.Common.
+Require Import Velus.Operators.
+Require Import Velus.NLustre.NLExprSyntax.
+Require Import Velus.SyBloc.SBSyntax.
+Require Import Velus.Clocks.
+
+Require Import Velus.RMemory.
+
+Require Import Velus.SyBloc.SBIsLast.
+
+Require Import List.
+Import List.ListNotations.
+Open Scope list_scope.
+
+Module Type SBMEMORYCORRES
+       (Import Ids     : IDS)
+       (Import Op      : OPERATORS)
+       (Import Clks    : CLOCKS       Ids)
+       (Import ExprSyn : NLEXPRSYNTAX     Op)
+       (Import Syn     : SBSYNTAX     Ids Op Clks ExprSyn)
+       (Import Last    : SBISLAST     Ids Op Clks ExprSyn Syn).
+
+  Definition state := memory val.
+  Definition menv := memory val.
+  Definition transient_states := Env.t (memory val).
+
+  Definition value_corres (x: ident) (S: state) (me: menv) : Prop :=
+    find_val x S = find_val x me.
+
+  Definition state_corres (s: ident) (S: state) (me: menv) : Prop :=
+    (forall Ss,
+        sub_inst s S Ss ->
+        exists me',
+          sub_inst s me me'
+          /\ me' ≋ Ss)
+    /\ forall me',
+      sub_inst s me me' ->
+      exists Ss,
+        sub_inst s S Ss.
+
+  Definition transient_state_corres (s: ident) (I: transient_states) (me: menv) : Prop :=
+    (forall Is,
+        Env.find s I = Some Is ->
+        exists me',
+          sub_inst s me me'
+          /\ me' ≋ Is)
+    /\ forall me',
+      sub_inst s me me' ->
+      exists Is,
+        Env.find s I = Some Is.
+
+  Definition Memory_Corres_eqs
+             (eqs: list equation)
+             (S: state) (I: transient_states) (S': state)
+             (me: menv) : Prop :=
+    (forall x,
+        (Is_last_in x eqs -> value_corres x S' me)
+        /\
+        (~ Is_last_in x eqs -> value_corres x S me))
+    /\
+    (forall s,
+        (~ Step_in s eqs /\ ~ Reset_in s eqs ->
+         state_corres s S me)
+        /\
+        (~ Step_in s eqs /\ Reset_in s eqs ->
+         transient_state_corres s I me)
+        /\
+        (Step_in s eqs ->
+         state_corres s S' me)).
+
+  Lemma Memory_Corres_eqs_Def:
+    forall x ck ce S I S' me eqs,
+      Memory_Corres_eqs eqs S I S' me ->
+      Memory_Corres_eqs (EqDef x ck ce :: eqs) S I S' me.
+  Proof.
+    intros ** (Lasts & Insts); split; [split|split; [|split]].
+    - inversion_clear 1 as [?? Last|]; eauto.
+      + inv Last.
+      + apply Lasts; auto.
+    - intro NLast; apply Lasts.
+      intro; apply NLast; right; auto.
+    - intros (Nstep & Nrst).
+      apply Insts; split.
+      + intro; apply Nstep; right; auto.
+      + intro; apply Nrst; right; auto.
+    - intros (Nstep & Rst).
+      apply Insts; split.
+      + intro; apply Nstep; right; auto.
+      + inversion_clear Rst as [?? IsSt|]; auto.
+        inv IsSt.
+    - intros Step.
+      apply Insts; inversion_clear Step as [?? IsSt|]; auto.
+      inv IsSt.
+  Qed.
+
+  Lemma Memory_Corres_eqs_Next_present:
+    forall x ck e S I S' me eqs c,
+      Memory_Corres_eqs eqs S I S' me ->
+      find_val x S' = Some c ->
+      Memory_Corres_eqs (EqNext x ck e :: eqs) S I S' (add_val x c me).
+  Proof.
+    intros ** (Lasts & Insts); split; [split|split; [|split]].
+    - inversion_clear 1 as [?? Last|?? Last]; eauto; unfold value_corres.
+      + inv Last; rewrite find_val_gss; auto.
+      + intros.
+        destruct (ident_eq_dec x0 x).
+        * subst; rewrite find_val_gss; auto.
+        * rewrite find_val_gso; auto;
+            apply Lasts with (1 := Last); auto.
+    - intros NLast **; unfold value_corres.
+      assert (x0 <> x)
+        by (intro; subst; apply NLast; left; constructor).
+      assert ( ~ Is_last_in x0 eqs)
+        by (intro; apply NLast; right; auto).
+      rewrite find_val_gso; auto;
+        apply Lasts; auto.
+    - intros (Nstep & Nrst).
+      assert (~ Step_in s eqs) by (intro; apply Nstep; right; auto).
+      assert (~ Reset_in s eqs) by (intro; apply Nrst; right; auto).
+      split; unfold sub_inst; setoid_rewrite find_inst_add_val;
+        apply Insts; auto.
+    - intros (Nstep & Rst).
+      assert (~ Step_in s eqs) by (intro; apply Nstep; right; auto).
+      assert (Reset_in s eqs)
+        by (inversion_clear Rst as [?? IsSt|]; auto; inv IsSt).
+      split; unfold sub_inst; setoid_rewrite find_inst_add_val;
+        apply Insts; auto.
+    - intros Step.
+      assert (Step_in s eqs)
+        by (inversion_clear Step as [?? IsSt|]; auto; inv IsSt).
+      split; unfold sub_inst; setoid_rewrite find_inst_add_val;
+        apply Insts; auto.
+  Qed.
+
+  Lemma Memory_Corres_eqs_Next_absent:
+    forall x ck e S I S' me eqs,
+      Memory_Corres_eqs eqs S I S' me ->
+      find_val x S' = find_val x S ->
+      Memory_Corres_eqs (EqNext x ck e :: eqs) S I S' me.
+  Proof.
+    intros ** (Lasts & Insts) Eq; split; [split|split; [|split]].
+    - inversion_clear 1 as [?? Last|?? Last]; eauto; unfold value_corres.
+      + inv Last.
+        destruct (Is_last_in_dec x eqs).
+        * apply Lasts; auto.
+        * setoid_rewrite Eq; apply Lasts; auto.
+      + apply Lasts; auto.
+    - intros NLast.
+      apply Lasts; intro; apply NLast; right; auto.
+    - intros (Nstep & Nrst).
+      apply Insts; split.
+      + intro; apply Nstep; right; auto.
+      + intro; apply Nrst; right; auto.
+    - intros (Nstep & Rst).
+      apply Insts; split.
+      + intro; apply Nstep; right; auto.
+      + inversion_clear Rst as [?? IsSt|]; auto.
+        inv IsSt.
+    - intros Step.
+      apply Insts; inversion_clear Step as [?? IsSt|]; auto.
+      inv IsSt.
+  Qed.
+
+  Lemma Memory_Corres_eqs_Reset_present:
+    forall s ck b S I S' Is me eqs me',
+      Memory_Corres_eqs eqs S I S' me ->
+      Env.find s I = Some Is ->
+      me' ≋ Is ->
+      ~ Step_in s eqs ->
+      Memory_Corres_eqs (EqReset s ck b :: eqs) S I S' (add_inst s me' me).
+  Proof.
+    intros ** (Lasts & Insts) ??; split; [split|split; [|split]].
+    - inversion_clear 1 as [?? Last|]; eauto.
+      + inv Last.
+      + apply Lasts; auto.
+    - intro NLast; apply Lasts.
+      intro; apply NLast; right; auto.
+    - intros (Nstep & Nrst).
+      assert (s0 <> s)
+        by (intro; subst; apply Nrst; left; constructor).
+      assert (~ Step_in s0 eqs) by (intro; apply Nstep; right; auto).
+      assert (~ Reset_in s0 eqs) by (intro; apply Nrst; right; auto).
+      split; unfold sub_inst; rewrite find_inst_gso; auto;
+        apply Insts; auto.
+    - intros (Nstep & Rst).
+      inversion_clear Rst as [?? Rst'|].
+      + inv Rst'.
+        split; unfold sub_inst; setoid_rewrite find_inst_gss.
+        * intros; exists me'; intuition; congruence.
+        * inversion 1; subst; intros; exists Is; eauto.
+      + destruct (ident_eq_dec s0 s).
+        *{ split; subst; unfold sub_inst; rewrite find_inst_gss.
+           - exists me'; intuition; congruence.
+           - inversion 1; subst; intros; exists Is; eauto.
+         }
+        * assert (~ Step_in s0 eqs) by (intro; apply Nstep; right; auto).
+          split; unfold sub_inst; rewrite find_inst_gso; auto;
+            apply (proj1 (proj2 (Insts s0))); auto.
+    - intros Step.
+      inversion_clear Step as [?? Step'|].
+      + inv Step'.
+      + destruct (ident_eq_dec s0 s).
+        * split; subst; intuition.
+        * split; unfold sub_inst; rewrite find_inst_gso; auto;
+            apply Insts; auto.
+  Qed.
+
+  Lemma Memory_Corres_eqs_Reset_absent:
+    forall s ck b S I S' Is Ss me eqs,
+      Memory_Corres_eqs eqs S I S' me ->
+      Env.find s I = Some Is ->
+      sub_inst s S Ss ->
+      Is ≋ Ss ->
+      ~ Reset_in s eqs ->
+      Memory_Corres_eqs (EqReset s ck b :: eqs) S I S' me.
+  Proof.
+    intros ** (Lasts & Insts) Find_I Find_S E; split; [split|split; [|split]].
+    - inversion_clear 1 as [?? Last|]; eauto.
+      + inv Last.
+      + apply Lasts; auto.
+    - intro NLast; apply Lasts.
+      intro; apply NLast; right; auto.
+    - intros (Nstep & Nrst).
+      apply Insts; split.
+      + intro; apply Nstep; right; auto.
+      + intro; apply Nrst; right; auto.
+    - intros (Nstep & Rst).
+      inversion_clear Rst as [?? Rst'|].
+      + inv Rst'.
+        assert (~ Step_in s eqs) by (intro; apply Nstep; right; auto).
+        split; unfold sub_inst.
+        * intros ** Find.
+          rewrite Find in Find_I; inv Find_I.
+          setoid_rewrite E.
+          apply (proj1 (Insts s)); auto.
+        * assert (state_corres s S me) as StCorr by (apply Insts; auto).
+          intros ** Find; apply StCorr in Find as (?& Find).
+          unfold sub_inst in *; rewrite Find in Find_S; inv Find_S.
+          exists Is; eauto.
+      + apply Insts; split; auto.
+        intro; apply Nstep; right; auto.
+    - intros Step.
+      inversion_clear Step as [?? Step'|].
+      + inv Step'.
+      + apply Insts; eauto.
+  Qed.
+
+  Lemma Memory_Corres_eqs_Call_present:
+    forall s ys ck (rst: bool) b es S I S' Ss' eqs me me',
+      Memory_Corres_eqs eqs S I S' me ->
+      sub_inst s S' Ss' ->
+      me' ≋ Ss' ->
+      Memory_Corres_eqs (EqCall s ys ck rst b es :: eqs) S I S' (add_inst s me' me).
+  Proof.
+    intros ** (Lasts & Insts) Find_S' E;
+      split; [split|split; [|split]].
+    - inversion_clear 1 as [?? Last|]; eauto.
+      + inv Last.
+      + apply Lasts; auto.
+    - intro NLast; apply Lasts.
+      intro; apply NLast; right; auto.
+    - intros (Nstep & Nrst).
+      assert (s0 <> s) as Neq
+          by (intro; subst; apply Nstep; left; constructor).
+      assert (~ Step_in s0 eqs) by (intro; apply Nstep; right; auto).
+      assert (~ Reset_in s0 eqs) by (intro; apply Nrst; right; auto).
+      split; unfold sub_inst; rewrite find_inst_gso; auto;
+        apply Insts; auto.
+    - intros (Nstep & Rst).
+      assert (s0 <> s) as Neq
+          by (intro; subst; apply Nstep; left; constructor).
+      assert (~ Step_in s0 eqs) by (intro; apply Nstep; right; auto).
+      inversion_clear Rst as [?? Rst'|]; try inv Rst'.
+      split; unfold sub_inst; rewrite find_inst_gso; auto;
+        apply Insts; auto.
+    - intros Step.
+      inversion_clear Step as [?? Step'|].
+      + inv Step'.
+        split; unfold sub_inst; rewrite find_inst_gss.
+        * exists me'; intuition; congruence.
+        * inversion 1; subst; exists Ss'; intuition.
+      + destruct (ident_eq_dec s0 s).
+        *{ split; subst; unfold sub_inst; rewrite find_inst_gss.
+           - exists me'; intuition; congruence.
+           - inversion 1; subst; exists Ss'; intuition.
+         }
+        * split; unfold sub_inst; rewrite find_inst_gso; auto;
+            apply Insts; auto.
+  Qed.
+
+  Lemma Memory_Corres_eqs_Call_absent:
+    forall s ys ck (rst: bool) b es S I S' Is Ss' eqs me,
+      Memory_Corres_eqs eqs S I S' me ->
+      Env.find s I = Some Is ->
+      (rst = false -> exists Ss, sub_inst s S Ss /\ Is ≋ Ss) ->
+      sub_inst s S' Ss' ->
+      Ss' ≋ Is ->
+      ~ Step_in s eqs /\ (if rst then Reset_in s eqs else ~ Reset_in s eqs) ->
+      Memory_Corres_eqs (EqCall s ys ck rst b es :: eqs) S I S' me.
+  Proof.
+    intros ** (Lasts & Insts) Find_I Find_S Find_S' E NstepRst;
+      split; [split|split; [|split]].
+    - inversion_clear 1 as [?? Last|]; eauto.
+      + inv Last.
+      + apply Lasts; auto.
+    - intro NLast; apply Lasts.
+      intro; apply NLast; right; auto.
+    - intros (Nstep & Nrst).
+      apply Insts; split.
+      + intro; apply Nstep; right; auto.
+      + intro; apply Nrst; right; auto.
+    - intros (Nstep & Rst).
+      apply Insts; split.
+      + intro; apply Nstep; right; auto.
+      + inversion_clear Rst as [?? Rst'|]; auto.
+        inv Rst'.
+    - intros Step.
+      inversion_clear Step as [?? Step'|].
+      + inv Step'.
+        destruct rst.
+        *{ apply Insts in Find_I as (me' & Sub &?); auto.
+           split; intros ** Sub'; unfold sub_inst in *.
+           - rewrite Find_S' in Sub'; inv Sub'.
+             exists me'; rewrite E; auto.
+           - rewrite Sub' in Sub; inv Sub.
+             exists Ss'; auto.
+         }
+        *{ destruct Find_S as (Ss & Find_S &?); auto.
+           apply Insts in Find_S as (me' & Sub &?); auto.
+           split; intros ** Sub'; unfold sub_inst in *.
+           - rewrite Find_S' in Sub'; inv Sub'.
+             exists me'; split; auto.
+             transitivity Ss; auto.
+             transitivity Is; symmetry; auto.
+           - rewrite Sub' in Sub; inv Sub.
+             exists Ss'; auto.
+         }
+      + apply Insts; eauto.
+  Qed.
+
+End SBMEMORYCORRES.
